Clean up exp/mexp mess, add nonmod bn exp

code/experimental/he/Hacl.Spec.HE.DGK.fst
@@ -101,61 +101,61 @@ let mod_product_zero a b p =
 // q /= 0 mod p, so k = 0 mod p,
 // so k = s * p,
 // so h^v = 1 + s*p*q
-val h_raise_v: p:prm -> q:prm{p <> q} -> v:pos -> h:fe (p*q){is_h p q v h} -> Lemma (fexp h v = 1)
+val h_raise_v: p:prm -> q:prm{p <> q} -> v:pos -> h:fe (p*q){is_h p q v h} -> Lemma (mexp h v = 1)
 let h_raise_v p q v h =
   swap_mul p q;
 
-  let l1 (): Lemma (fexp h v = 1 + (fexp h v / p) * p /\
-                    fexp h v = 1 + (fexp h v / q) * q) = begin
+  let l1 (): Lemma (mexp h v = 1 + (mexp h v / p) * p /\
+                    mexp h v = 1 + (mexp h v / q) * q) = begin
     isunit_comp p q h;
 
     multiple_modulo_lemma p q;
     multiple_division_lemma p q;
-    to_fe_fexp1 #(p*q) q h v;
-    mod_prop p (fexp h v) 1;
+    to_fe_mexp1 #(p*q) q h v;
+    mod_prop p (mexp h v) 1;
 
     multiple_modulo_lemma q p;
     multiple_division_lemma q p;
-    to_fe_fexp1 #(p*q) p h v;
-    mod_prop q (fexp h v) 1
+    to_fe_mexp1 #(p*q) p h v;
+    mod_prop q (mexp h v) 1
     end in
 
   l1 ();
 
-  let l2 (): Lemma (fexp h v = 1 + ((fexp h v / p) / q) * (p * q)) = begin
-    assert (fexp h v - fexp h v = (1 + (fexp h v / p) * p) - (1 + (fexp h v / q) * q));
-    assert (0 = (fexp h v / p) * p - (fexp h v / q) * q);
-    assert (0 % q = ((fexp h v / p) * p - (fexp h v / q) * q) % q);
+  let l2 (): Lemma (mexp h v = 1 + ((mexp h v / p) / q) * (p * q)) = begin
+    assert (mexp h v - mexp h v = (1 + (mexp h v / p) * p) - (1 + (mexp h v / q) * q));
+    assert (0 = (mexp h v / p) * p - (mexp h v / q) * q);
+    assert (0 % q = ((mexp h v / p) * p - (mexp h v / q) * q) % q);
 
     small_mod 0 q;
 
-    modulo_distributivity ((fexp h v / p) * p) (- (fexp h v / q) * q) q;
+    modulo_distributivity ((mexp h v / p) * p) (- (mexp h v / q) * q) q;
 
-    assert (0 = (((fexp h v / p) * p) % q - ((fexp h v / q) * q) % q) % q);
+    assert (0 = (((mexp h v / p) * p) % q - ((mexp h v / q) * q) % q) % q);
 
-    multiple_modulo_lemma (fexp h v / q) q;
-    assert (0 = (((fexp h v / p) * p) % q) % q);
+    multiple_modulo_lemma (mexp h v / q) q;
+    assert (0 = (((mexp h v / p) * p) % q) % q);
 
-    modulo_modulo_lemma ((fexp h v / p) * p) q 1;
-    assert (((fexp h v / p) * p) % q = 0);
+    modulo_modulo_lemma ((mexp h v / p) * p) q 1;
+    assert (((mexp h v / p) * p) % q = 0);
 
-    mod_product_zero (fexp h v / p) p q;
-    assert ((fexp h v / p) % q = 0);
+    mod_product_zero (mexp h v / p) p q;
+    assert ((mexp h v / p) % q = 0);
 
-    mod_prop q (fexp h v / p) 0;
-    assert (fexp h v / p = ((fexp h v / p) / q) * q);
+    mod_prop q (mexp h v / p) 0;
+    assert (mexp h v / p = ((mexp h v / p) / q) * q);
 
-    assert (fexp h v = 1 + ((fexp h v / p) / q) * q * p);
-    paren_mul_right ((fexp h v / p) / q) q p
+    assert (mexp h v = 1 + ((mexp h v / p) / q) * q * p);
+    paren_mul_right ((mexp h v / p) / q) q p
   end in
 
   l2 ();
 
-  mod_prop_inv (p * q) (fexp h v) 1 ((fexp h v / p) / q);
+  mod_prop_inv (p * q) (mexp h v) 1 ((mexp h v / p) / q);
   small_mod 1 (p * q);
-  to_fe_idemp #(p * q) (fexp h v);
+  to_fe_idemp #(p * q) (mexp h v);
 
-  assert (fexp h v = 1)
+  assert (mexp h v = 1)
 
 #reset-options
 
@@ -169,21 +169,6 @@ val solve_dlp_power:
   -> a:fe n
   -> x:fe (exp p s)
 let solve_dlp_power #n u g a = admit()
-
-// Inverting an element of Z_p using fermat inverse theorem.
-val fermat_inverse_unit:
-     p:prm
-  -> a:fe p{isunit a}
-  -> b:fe p{isunit b /\ a *% b = 1 /\ b = finv a}
-let fermat_inverse_unit p a =
-  let b = fexp a (p - 2) in
-
-  fexp_mul1 a (p - 2) 1;
-  fexp_one1 a;
-  flt a;
-  finv_unique #p a b;
-
-  b
 
 
 type is_crt_base (base:S.seq (tuple2 prm pos)) =
@@ -219,11 +204,12 @@ val fermat_inv_pe:
   -> a:fe (exp p e)
   -> b:fe (exp p e) {isunit a ==> (isunit b /\ a *% b = 1 /\ b = finv a)}
 let fermat_inv_pe p e a =
-  let b = fexp a (carm_pe p e - 1) in
+  let lam = carm_pe p e in
+  let b = mexp a (lam - 1) in
 
-  fexp_mul1 a (carm_pe p e - 1) 1;
-  fexp_one1 a;
-  euler_thm (exp p e) (pe_fact p e) (carm_pe p e) a;
+  mexp_mul1 a (lam - 1) 1;
+  mexp_one1 a;
+  euler_thm (exp p e) (pe_fact p e) lam a;
   finv_unique #(exp p e) a b;
 
   b
@@ -313,13 +299,13 @@ val encrypt:
   -> r:pos
   -> m:fe (Public?.u p)
   -> c:ciphertext (Public?.n p)
-let encrypt p r m = fexp (Public?.g p) m *% fexp (Public?.h p) r
+let encrypt p r m = mexp (Public?.g p) m *% mexp (Public?.h p) r
 
 val check_is_zero:
      s:secret
   -> c:ciphertext (Public?.n (s2p s))
   -> bool
-let check_is_zero s c = fexp c (Secret?.v s) = 1
+let check_is_zero s c = mexp c (Secret?.v s) = 1
 
 val check_is_zero_prop:
      s:secret
@@ -333,26 +319,26 @@ let check_is_zero_prop s r m =
   let v = Secret?.v s in
   let u = Secret?.u s in
   let c = encrypt (s2p s) r m in
-  let gv = fexp g v in
-  let cv = fexp c v in
-  fexp_mul2 (fexp g m) (fexp h r) v;
-  fexp_exp h r v;
-  fexp_exp h v r;
+  let gv = mexp g v in
+  let cv = mexp c v in
+  mexp_mul2 (mexp g m) (mexp h r) v;
+  mexp_exp h r v;
+  mexp_exp h v r;
   h_raise_v (Secret?.p s) (Secret?.q s) v h;
-  fexp_exp g m v;
-  fexp_exp g v m;
-  assert (fexp c v = fexp gv m);
+  mexp_exp g m v;
+  mexp_exp g v m;
+  assert (mexp c v = mexp gv m);
 
-  let g_pow_nonzero (x:nat): Lemma (fexp g x <> 0) = begin
+  let g_pow_nonzero (x:nat): Lemma (mexp g x <> 0) = begin
     g_pow_isunit g x;
-    isunit_nonzero (fexp g x)
+    isunit_nonzero (mexp g x)
   end in
 
   g_pow_nonzero v;
   nat_times_nat_is_nat v m;
   g_pow_nonzero (v * m);
 
-  fexp_zero2 gv;
+  mexp_zero2 gv;
   assert (m = 0 ==> check_is_zero s (encrypt (s2p s) r m) = true);
 
   let m_neq_zero (): Lemma (requires m <> 0)
@@ -374,7 +360,7 @@ let decrypt s c =
   let g = Secret?.g s in
   let v = Secret?.v s in
   let u = Secret?.u s in
-  let gv = fexp g v in
+  let gv = mexp g v in
   g_pow_isunit g v;
-  mult_order_of_fexp g v u;
-  solve_dlp (Secret?.u s) gv (fexp c (Secret?.v s))
+  mult_order_of_mexp g v u;
+  solve_dlp (Secret?.u s) gv (mexp c (Secret?.v s))
