code/experimental/rsapss/Hacl.Impl.Bignum.Modular.fst
@@ -260,3 +260,71 @@ let bn_modular_mul #len n a b res =
   bn_mul a b res';
   bn_remainder res' n res;
   pop_frame ()
+
+
+#reset-options "--z3rlimit 100 --max_fuel 0 --max_ifuel 0 --using_facts_from '* -FStar.Seq'"
+
+val naive_mod_exp_loop:
+     #nLen:bn_len_strict{(v nLen + v nLen) * 64 < max_size_t}
+  -> #expLen:bn_len_strict
+  -> n:lbignum nLen
+  -> a:lbignum nLen
+  -> b:lbignum expLen
+  -> res:lbignum nLen
+  -> Stack unit
+    (requires fun h ->
+        disjoint n b /\ disjoint n res /\
+        live h n /\ live h a /\ live h b /\ live h res /\
+        as_snat h n > 1)
+    (ensures fun h0 _ h1 -> modifies2 res b h0 h1 /\
+        live h1 n /\ live h1 a /\ live h1 b /\ live h1 res)
+let rec naive_mod_exp_loop #nLen #expLen n a b res =
+  push_frame ();
+  let tmp = create expLen (uint 0) in
+  let tmp' = create nLen (uint 0) in
+  assert_norm (issnat 0);
+  assert_norm (nat_bytes_num 0 =. 1ul);
+  let zero:lbignum 1ul = nat_to_bignum_exact 0 in
+  let isnull = bn_is_equal b zero in
+  if not isnull then begin
+     let odd = eq_u64 (b.(0ul) &. uint 1) (uint 1) in
+     bn_rshift1 b tmp; copy b tmp;
+     naive_mod_exp_loop #nLen n a b res;
+     bn_modular_mul n res res tmp'; copy res tmp';
+     if odd then (bn_modular_mul n res a tmp'; copy res tmp')
+  end;
+  pop_frame ()
+
+val bn_modular_exp:
+     #nLen:bn_len_strict{v nLen * 128 < max_size_t}
+  -> #expLen:bn_len_strict
+  -> n:lbignum nLen
+  -> a:lbignum nLen
+  -> b:lbignum expLen
+  -> res:lbignum nLen
+  -> Stack unit
+    (requires fun h ->
+      live h n /\ live h a /\ live h b /\ live h res /\
+      disjoint a res /\ disjoint b res /\ disjoint n res /\
+      as_snat h n > 1)
+    (ensures  fun h0 _ h1 -> modifies1 res h0 h1 /\
+      live h1 n /\ live h1 a /\ live h1 b /\ live h1 res /\
+      (let n = as_snat h0 n in
+       as_snat h1 res = mexp (to_fe #n (as_snat h0 a)) (as_snat h0 b)))
+let bn_modular_exp #nLen #expLen n a b res =
+  let h0 = FStar.HyperStack.ST.get () in
+
+  push_frame ();
+
+  memset res (uint 0) nLen;
+  res.(0ul) <- uint 1;
+  let tmp_b = create expLen (uint 0) in
+  copy tmp_b b;
+  naive_mod_exp_loop n a tmp_b res;
+
+  pop_frame ();
+
+  let h1 = FStar.HyperStack.ST.get () in
+  assume (let n' = as_snat h0 n in
+          as_snat h1 res =
+          mexp (to_fe #n' (as_snat h0 a)) (as_snat h0 b))
